Resolve function declarations

src/Ast/Resolver.dfy
@@ -13,6 +13,24 @@ module Resolver {
   method Resolve(b3: Raw.Program) returns (r: Result<Ast.Program, string>)
     ensures r.Success? ==> b3.WellFormed() && r.value.WellFormed()
   {
+    var typeMap :- ResolveAllTypes(b3);
+    var functionMap :- ResolveAllFunctions(b3, typeMap);
+    var ers := ExprResolverState(b3, typeMap, functionMap);
+    var procMap :- ResolveAllProcedures(ers);
+
+    var r3 := Program(typeMap.Values, procMap.Values);
+
+    return Success(r3);
+  }
+
+  method ResolveAllTypes(b3: Raw.Program) returns (r: Result<map<string, TypeDecl>, string>)
+    ensures r.Success? ==> var typeMap := r.value;
+      && typeMap.Keys == (set typename <- b3.types)
+      && MapIsInjective(typeMap)
+      && (forall typename <- typeMap.Keys :: typeMap[typename].Name == typename)
+      && (forall typename <- b3.types :: typename !in BuiltInTypes)
+      && (forall i, j :: 0 <= i < j < |b3.types| ==> b3.types[i] != b3.types[j])
+  {
     var typeMap: map<string, TypeDecl> := map[];
     for n := 0 to |b3.types|
       // typeMap maps user-defined types seen so far to distinct type-declaration objects
@@ -27,14 +45,145 @@ module Resolver {
     {
       var name := b3.types[n];
       if name in BuiltInTypes {
-        return Failure("user-defined type is not allowed to have the name of a built-in type: " + name);
+        return Result<map<string, TypeDecl>, string>.Failure("user-defined type is not allowed to have the name of a built-in type: " + name);
       } else if name in typeMap.Keys {
         return Failure("duplicate type name: " + name);
       }
       var decl := new TypeDecl(name);
       typeMap := typeMap[name := decl];
     }
+    return Success(typeMap);
+  }
 
+  method ResolveAllFunctions(b3: Raw.Program, typeMap: map<string, TypeDecl>) returns (r: Result<map<string, Function>, string>)
+    requires forall typename :: b3.IsType(typename) <==> typename in BuiltInTypes || typename in typeMap
+    ensures r.Success? ==>
+      && (forall i, j :: 0 <= i < j < |b3.functions| ==> b3.functions[i].name != b3.functions[j].name)
+      && (forall func <- b3.functions :: func.WellFormed(b3))
+    ensures r.Success? ==> var functions: set<Function> := r.value.Values;
+      && (forall func0 <- functions, func1 <- functions :: func0.Name == func1.Name ==> func0 == func1)
+      && (forall func <- functions :: func.WellFormed())
+    ensures r.Success? ==> var functionMap := r.value;
+      && (forall functionName <- functionMap :: exists func <- b3.functions :: func.name == functionName)
+      && (forall rawFunction <- b3.functions ::
+            && rawFunction.name in functionMap
+            && var func := functionMap[rawFunction.name];
+            && |rawFunction.parameters| == |func.Parameters|
+         )
+  {
+    var functionMap: map<string, Function> := map[];
+    for n := 0 to |b3.functions|
+      // functionMap maps the user-defined functions seen so far to distinct and fresh function-declaration objects
+      invariant functionMap.Keys == set func <- b3.functions[..n] :: func.name
+      invariant MapIsInjective(functionMap)
+      invariant forall name <- functionMap :: fresh(functionMap[name])
+      // functionMap organizes function-declaration objects correctly according to their names
+      invariant forall functionName <- functionMap.Keys :: functionMap[functionName].Name == functionName
+      // functions seen so far have distinct names
+      invariant forall i, j :: 0 <= i < j < n ==> b3.functions[i].name != b3.functions[j].name
+      // the functions seen so far are well-formed
+      invariant forall func <- b3.functions[..n] :: func.SignatureWellFormed(b3) && functionMap[func.name].SignatureWellFormed(func)
+    {
+      var func := b3.functions[n];
+      var name := func.name;
+      if name in functionMap.Keys {
+        return Failure("duplicate function name: " + name);
+      }
+      var rfunc :- ResolveFunctionSignature(func, b3, typeMap);
+      functionMap := functionMap[name := rfunc];
+    }
+
+    var ers := ExprResolverState(b3, typeMap, functionMap);
+    for n := 0 to |b3.functions|
+      invariant forall func <- b3.functions :: func.SignatureWellFormed(b3) && functionMap[func.name].SignatureWellFormed(func)
+      invariant forall func <- b3.functions[..n] :: func.WellFormed(b3)
+      invariant forall func <- b3.functions[..n] :: functionMap[func.name].WellFormed()
+    {
+      var func := b3.functions[n];
+      var _ :- ResolveFunction(func, functionMap[func.name], ers);
+    }
+
+    return Success(functionMap);
+  }
+
+  method ResolveFunctionSignature(func: Raw.Function, b3: Raw.Program, typeMap: map<string, TypeDecl>) returns (r: Result<Function, string>)
+    requires forall typename :: b3.IsType(typename) <==> typename in BuiltInTypes || typename in typeMap
+    ensures r.Success? ==> func.SignatureWellFormed(b3)
+    ensures r.Success? ==> fresh(r.value) && r.value.SignatureWellFormed(func)
+  {
+    var paramMap: map<string, Variable> := map[];
+    var formals: seq<FParameter> := [];
+    for n := 0 to |func.parameters|
+      invariant forall p <- func.parameters[..n] :: Raw.LegalVariableName(p.name) && b3.IsType(p.typ)
+      invariant forall i, j :: 0 <= i < j < n ==> func.parameters[i].name != func.parameters[j].name
+      invariant paramMap.Keys == (set p <- func.parameters[..n] :: p.name)
+      invariant |formals| == n
+      invariant forall i :: 0 <= i < n ==> formals[i] == paramMap[func.parameters[i].name]
+      invariant forall i :: 0 <= i < n ==> formals[i].name == func.parameters[i].name
+      invariant forall i :: 0 <= i < n ==> formals[i].injective == func.parameters[i].injective
+    {
+      var p := func.parameters[n];
+      if !Raw.LegalVariableName(p.name) {
+        return Failure("illegal parameter name: " + p.name);
+      }
+      if p.name in paramMap {
+        return Failure("duplicate parameter name: " + p.name);
+      }
+      var typ :- ResolveType(p.typ, typeMap);
+
+      var formal: FParameter := new FParameter(p.name, p.injective, typ);
+      paramMap := paramMap[p.name := formal];
+      formals := formals + [formal];
+    }
+
+    var rfunc := new Function(func.name, formals);
+    return Success(rfunc);
+  }
+
+  method ResolveFunction(func: Raw.Function, rfunc: Function, ers: ExprResolverState) returns (r: Result<(), string>)
+    requires func.SignatureWellFormed(ers.b3) && rfunc.SignatureWellFormed(func) && ers.Valid()
+    modifies rfunc
+    ensures r.Success? ==> func.WellFormed(ers.b3) && rfunc.WellFormed()
+  {
+    if func.definition == None {
+      rfunc.Definition := None;
+      return Success(());
+    }
+
+    var formals := rfunc.Parameters;
+    var n := |formals|;
+    assert forall formal: FParameter <- formals :: Raw.LegalVariableName(formal.name);
+    assert forall i, j :: 0 <= i < j < n ==> formals[i].name != formals[j].name;
+    var paramMap := map formal <- rfunc.Parameters :: formal.name := formal;
+
+    assert n == |func.parameters|;
+    assert forall i :: 0 <= i < n ==> formals[i].name == func.parameters[i].name;
+
+    var bodyScope := set p <- func.parameters :: p.name;
+    var whenScope := bodyScope;
+
+    var whenVariables := MapProject(paramMap, whenScope);
+    assert whenVariables.Keys == whenScope;
+    var when :- ResolveExprList(func.definition.value.when, ers, whenVariables);
+
+    var bodyVariables := MapProject(paramMap, bodyScope);
+    assert bodyVariables.Keys == bodyScope;
+    var body :- ResolveExpr(func.definition.value.body, ers, bodyVariables);
+
+    rfunc.Definition := Some(FunctionDefinition(when, body));
+    return Success(());
+  }
+
+  method ResolveAllProcedures(ers: ExprResolverState) returns (r: Result<map<string, Procedure>, string>)
+    requires ers.Valid()
+    ensures r.Success? ==>
+      && (forall i, j :: 0 <= i < j < |ers.b3.procedures| ==> ers.b3.procedures[i].name != ers.b3.procedures[j].name)
+      && (forall proc <- ers.b3.procedures :: proc.WellFormed(ers.b3))
+    ensures r.Success? ==> var procedures: set<Procedure> := r.value.Values;
+      && (forall proc0 <- procedures, proc1 <- procedures :: proc0.Name == proc1.Name ==> proc0 == proc1)
+      && (forall proc <- procedures :: proc.WellFormed())
+  {
+    var b3 := ers.b3;
     var procMap: map<string, Procedure> := map[];
     for n := 0 to |b3.procedures|
       // procMap maps the user-defined procedures seen so far to distinct and fresh procedure-declaration objects
@@ -47,40 +196,39 @@ module Resolver {
       invariant forall i, j :: 0 <= i < j < n ==> b3.procedures[i].name != b3.procedures[j].name
       // the procedures seen so far are well-formed
       invariant forall proc <- b3.procedures[..n] :: proc.SignatureWellFormed(b3) && procMap[proc.name].SignatureWellFormed(proc)
-    {
+   {
       var proc := b3.procedures[n];
       var name := proc.name;
       if name in procMap.Keys {
         return Failure("duplicate procedure name: " + name);
       }
-      var rproc :- ResolveProcedureSignature(proc, b3, typeMap);
+      var rproc :- ResolveProcedureSignature(proc, ers);
       procMap := procMap[name := rproc];
     }
 
-    var rs := ResolverState(b3, typeMap, procMap);
+    var prs := ProcResolverState(ers, procMap);
+    assert prs.Valid(); // TODO: this assert is probably not needed
     for n := 0 to |b3.procedures|
       invariant forall proc <- b3.procedures :: proc.SignatureWellFormed(b3) && procMap[proc.name].SignatureWellFormed(proc)
       invariant forall proc <- b3.procedures[..n] :: proc.WellFormed(b3)
       invariant forall proc <- b3.procedures[..n] :: procMap[proc.name].WellFormed()
     {
       var proc := b3.procedures[n];
-      var _ :- ResolveProcedure(proc, procMap[proc.name], rs);
+      var _ :- ResolveProcedure(proc, procMap[proc.name], prs);
     }
 
-    var r3 := Program(typeMap.Values, procMap.Values);
-
-    return Success(r3);
+    return Success(procMap);
   }
 
-  method ResolveProcedureSignature(proc: Raw.Procedure, b3: Raw.Program, typeMap: map<string, TypeDecl>) returns (r: Result<Procedure, string>)
-    requires forall typename :: b3.IsType(typename) <==> typename in BuiltInTypes || typename in typeMap
-    ensures r.Success? ==> proc.SignatureWellFormed(b3)
+  method ResolveProcedureSignature(proc: Raw.Procedure, ers: ExprResolverState) returns (r: Result<Procedure, string>)
+    requires ers.Valid()
+    ensures r.Success? ==> proc.SignatureWellFormed(ers.b3)
     ensures r.Success? ==> fresh(r.value) && r.value.SignatureWellFormed(proc)
   {
     var paramMap: map<string, Variable> := map[];
     var formals: seq<Parameter> := [];
     for n := 0 to |proc.parameters|
-      invariant forall p <- proc.parameters[..n] :: Raw.LegalVariableName(p.name) && b3.IsType(p.typ)
+      invariant forall p <- proc.parameters[..n] :: Raw.LegalVariableName(p.name) && ers.b3.IsType(p.typ)
       invariant forall i, j :: 0 <= i < j < n ==> proc.parameters[i].name != proc.parameters[j].name
       invariant paramMap.Keys ==
         (set p <- proc.parameters[..n] :: p.name) +
@@ -98,7 +246,7 @@ module Resolver {
       if p.name in paramMap {
         return Failure("duplicate parameter name: " + p.name);
       }
-      var typ :- ResolveType(p.typ, typeMap);
+      var typ :- ResolveType(p.typ, ers.typeMap);
 
       var oldInOut;
       if p.mode == Raw.InOut {
@@ -133,16 +281,29 @@ module Resolver {
     return Success(UserType(typeMap[typename]));
   }
 
-  datatype ResolverState = ResolverState(b3: Raw.Program, typeMap: map<string, TypeDecl>, procMap: map<string, Procedure>)
+  datatype ProcResolverState = ProcResolverState(ers: ExprResolverState, procMap: map<string, Procedure>)
+  {
+    ghost predicate Valid() {
+      && ers.Valid()
+      && (forall procname <- procMap :: exists proc <- ers.b3.procedures :: proc.name == procname)
+      && (forall rawProc <- ers.b3.procedures ::
+            && rawProc.name in procMap
+            && var proc := procMap[rawProc.name];
+            && |rawProc.parameters| == |proc.Parameters|
+            && (forall i :: 0 <= i < |rawProc.parameters| ==> rawProc.parameters[i].mode == proc.Parameters[i].mode)
+         )
+    }
+  }
+
+  datatype ExprResolverState = ExprResolverState(b3: Raw.Program, typeMap: map<string, TypeDecl>, functionMap: map<string, Function>)
   {
     ghost predicate Valid() {
       && (forall typename :: b3.IsType(typename) <==> typename in BuiltInTypes || typename in typeMap)
-      && (forall procname <- procMap :: exists proc <- b3.procedures :: proc.name == procname)
-      && (forall rawProc <- b3.procedures ::
-            rawProc.name in procMap &&
-            var proc := procMap[rawProc.name];
-            && |rawProc.parameters| == |proc.Parameters|
-            && (forall i :: 0 <= i < |rawProc.parameters| ==> rawProc.parameters[i].mode == proc.Parameters[i].mode)
+      && (forall functionName <- functionMap :: exists func <- b3.functions :: func.name == functionName)
+      && (forall rawFunction <- b3.functions ::
+            && rawFunction.name in functionMap
+            && var func := functionMap[rawFunction.name];
+            && |rawFunction.parameters| == |func.Parameters|
          )
     }
   }
@@ -188,10 +349,10 @@ module Resolver {
     }
   }
 
-  method ResolveProcedure(proc: Raw.Procedure, rproc: Procedure, rs: ResolverState) returns (r: Result<(), string>)
-    requires proc.SignatureWellFormed(rs.b3) && rproc.SignatureWellFormed(proc) && rs.Valid()
+  method ResolveProcedure(proc: Raw.Procedure, rproc: Procedure, prs: ProcResolverState) returns (r: Result<(), string>)
+    requires proc.SignatureWellFormed(prs.ers.b3) && rproc.SignatureWellFormed(proc) && prs.Valid()
     modifies rproc
-    ensures r.Success? ==> proc.WellFormed(rs.b3) && rproc.WellFormed()
+    ensures r.Success? ==> proc.WellFormed(prs.ers.b3) && rproc.WellFormed()
   {
     var formals := rproc.Parameters;
     var n := |formals|;
@@ -220,18 +381,18 @@ module Resolver {
 
     var preVariables := MapProject(paramMap, preScope);
     assert preVariables.Keys == preScope;
-    var pre :- ResolveAExprs(proc.pre, rs, LocalResolverState(preVariables, map[], None, returnLabel));
+    var pre :- ResolveAExprs(proc.pre, prs, LocalResolverState(preVariables, map[], None, returnLabel));
 
     var postVariables := MapProject(paramMap, postScope);
     assert postVariables.Keys == postScope;
     var ls := LocalResolverState(postVariables, map[], None, returnLabel);
-    var post :- ResolveAExprs(proc.post, rs, ls);
+    var post :- ResolveAExprs(proc.post, prs, ls);
 
     var body;
     if proc.body == None {
       body := None;
     } else {
-      var b :- ResolveStmt(proc.body.value, rs, ls);
+      var b :- ResolveStmt(proc.body.value, prs, ls);
       body := Some(LabeledStmt(returnLabel, b));
     }
 
@@ -241,39 +402,39 @@ module Resolver {
     return Success(());
   }
 
-  method ResolveAExprs(aexprs: seq<Raw.AExpr>, rs: ResolverState, ls: LocalResolverState) returns (r: Result<seq<AExpr>, string>)
-    requires rs.Valid()
-    ensures r.Success? ==> forall ae <- aexprs :: ae.WellFormed(rs.b3, ls.varMap.Keys)
+  method ResolveAExprs(aexprs: seq<Raw.AExpr>, prs: ProcResolverState, ls: LocalResolverState) returns (r: Result<seq<AExpr>, string>)
+    requires prs.Valid()
+    ensures r.Success? ==> forall ae <- aexprs :: ae.WellFormed(prs.ers.b3, ls.varMap.Keys)
     ensures r.Success? ==> forall ae <- r.value :: ae.WellFormed()
   {
     var result := [];
     for n := 0 to |aexprs|
-      invariant forall ae <- aexprs[..n] :: ae.WellFormed(rs.b3, ls.varMap.Keys)
+      invariant forall ae <- aexprs[..n] :: ae.WellFormed(prs.ers.b3, ls.varMap.Keys)
       invariant forall ae: AExpr <- result :: ae.WellFormed()
     {
-      var ae :- ResolveAExpr(aexprs[n], rs, ls);
+      var ae :- ResolveAExpr(aexprs[n], prs, ls);
       result := result + [ae];
     }
     return Success(result);
   }
 
-  method ResolveAExpr(aexpr: Raw.AExpr, rs: ResolverState, ls: LocalResolverState) returns (r: Result<AExpr, string>)
-    requires rs.Valid()
-    ensures r.Success? ==> aexpr.WellFormed(rs.b3, ls.varMap.Keys)
+  method ResolveAExpr(aexpr: Raw.AExpr, prs: ProcResolverState, ls: LocalResolverState) returns (r: Result<AExpr, string>)
+    requires prs.Valid()
+    ensures r.Success? ==> aexpr.WellFormed(prs.ers.b3, ls.varMap.Keys)
     ensures r.Success? ==> r.value.WellFormed()
   {
     match aexpr
     case AExpr(e) =>
-      var expr :- ResolveExpr(e, rs, ls.varMap);
+      var expr :- ResolveExpr(e, prs.ers, ls.varMap);
       return Success(AExpr(expr));
     case AAssertion(s) =>
-      var stmt :- ResolveStmt(s, rs, ls.(labelMap := map[], loopLabel := None));
+      var stmt :- ResolveStmt(s, prs, ls.(labelMap := map[], loopLabel := None));
       return Success(AAssertion(stmt));
   }
 
-  method ResolveStmt(stmt: Raw.Stmt, rs: ResolverState, ls: LocalResolverState) returns (result: Result<Stmt, string>)
-    requires rs.Valid()
-    ensures result.Success? ==> stmt.WellFormed(rs.b3, ls.varMap.Keys, ls.LabelSet(), ls.loopLabel.Some?)
+  method ResolveStmt(stmt: Raw.Stmt, prs: ProcResolverState, ls: LocalResolverState) returns (result: Result<Stmt, string>)
+    requires prs.Valid()
+    ensures result.Success? ==> stmt.WellFormed(prs.ers.b3, ls.varMap.Keys, ls.LabelSet(), ls.loopLabel.Some?)
     ensures result.Success? ==> result.value.WellFormed()
   {
     var r: Stmt;
@@ -282,18 +443,18 @@ module Resolver {
         if !Raw.LegalVariableName(variable.name) {
           return Failure("illegal variable name: " + variable.name);
         }
-        var typ :- ResolveType(variable.typ, rs.typeMap);
+        var typ :- ResolveType(variable.typ, prs.ers.typeMap);
         var v := new LocalVariable(variable.name, variable.isMutable, typ);
         var i;
         if init == None {
           i := None;
         } else {
-          var e :- ResolveExpr(init.value, rs, ls.varMap);
+          var e :- ResolveExpr(init.value, prs.ers, ls.varMap);
           i := Some(e);
         }
         var ls' := ls.AddVariable(variable.name, v);
         assert ls'.varMap.Keys == ls.varMap.Keys + {v.name};
-        var b :- ResolveStmt(body, rs, ls');
+        var b :- ResolveStmt(body, prs, ls');
         r := VarDecl(v, i, b);
 
       case Assign(lhs, rhs) =>
@@ -301,48 +462,48 @@ module Resolver {
           return Failure("undeclared variable: " + lhs);
         }
         var left := ls.varMap[lhs];
-        var right :- ResolveExpr(rhs, rs, ls.varMap);
+        var right :- ResolveExpr(rhs, prs.ers, ls.varMap);
         r := Assign(left, right);
 
       case Block(stmts) =>
         var ss := [];
         for n := 0 to |stmts|
-          invariant forall stmt <- stmts[..n] :: stmt.WellFormed(rs.b3, ls.varMap.Keys, ls.LabelSet(), ls.loopLabel.Some?)
+          invariant forall stmt <- stmts[..n] :: stmt.WellFormed(prs.ers.b3, ls.varMap.Keys, ls.LabelSet(), ls.loopLabel.Some?)
           invariant forall stmt: Stmt <- ss :: stmt.WellFormed()
         {
-          var s :- ResolveStmt(stmts[n], rs, ls);
+          var s :- ResolveStmt(stmts[n], prs, ls);
           ss := ss + [s];
         }
         r := Block(ss);
 
       case Call(_, _) =>
-        r :- ResolveCallStmt(stmt, rs, ls);
+        r :- ResolveCallStmt(stmt, prs, ls);
 
       case Check(cond) =>
-        var c :- ResolveExpr(cond, rs, ls.varMap);
+        var c :- ResolveExpr(cond, prs.ers, ls.varMap);
         r := Check(c);
 
       case Assume(cond) =>
-        var c :- ResolveExpr(cond, rs, ls.varMap);
+        var c :- ResolveExpr(cond, prs.ers, ls.varMap);
         r := Assume(c);
 
       case Assert(cond) =>
-        var c :- ResolveExpr(cond, rs, ls.varMap);
+        var c :- ResolveExpr(cond, prs.ers, ls.varMap);
         r := Assert(c);
 
       case AForall(name, typ, body) =>
         if !Raw.LegalVariableName(name) {
           return Failure("illegal variable name: " + name);
         }
-        var t :- ResolveType(typ, rs.typeMap);
+        var t :- ResolveType(typ, prs.ers.typeMap);
         var v := new LocalVariable(name, false, t);
-        var b :- ResolveStmt(body, rs, ls.AddVariable(name, v));
+        var b :- ResolveStmt(body, prs, ls.AddVariable(name, v));
         r := AForall(v, b);
 
       case If(cond, thn, els) =>
-        var c :- ResolveExpr(cond, rs, ls.varMap);
-        var th :- ResolveStmt(thn, rs, ls);
-        var el :- ResolveStmt(els, rs, ls);
+        var c :- ResolveExpr(cond, prs.ers, ls.varMap);
+        var th :- ResolveStmt(thn, prs, ls);
+        var el :- ResolveStmt(els, prs, ls);
         var branch0 := PrependAssumption(c, th);
         var branch1 := PrependAssumption(Expr.CreateNegation(c), el);
         r := Choice([branch0, branch1]);
@@ -354,27 +515,27 @@ module Resolver {
         var branches := [];
         for n := 0 to |cases|
           invariant forall cs <- cases[..n] ::
-            && cs.cond.WellFormed(rs.b3, ls.varMap.Keys)
-            && cs.body.WellFormed(rs.b3, ls.varMap.Keys, ls.LabelSet(), ls.loopLabel.Some?)
+            && cs.cond.WellFormed(prs.ers.b3, ls.varMap.Keys)
+            && cs.body.WellFormed(prs.ers.b3, ls.varMap.Keys, ls.LabelSet(), ls.loopLabel.Some?)
           invariant forall branch: Stmt <- branches :: branch.WellFormed()
         {
-          var cond :- ResolveExpr(cases[n].cond, rs, ls.varMap);
-          var body :- ResolveStmt(cases[n].body, rs, ls);
+          var cond :- ResolveExpr(cases[n].cond, prs.ers, ls.varMap);
+          var body :- ResolveStmt(cases[n].body, prs, ls);
           branches := branches + [PrependAssumption(cond, body)];
         }
         r := Choice(branches);
 
       case Loop(invariants, body) =>
-        var invs :- ResolveAExprs(invariants, rs, ls);
+        var invs :- ResolveAExprs(invariants, prs, ls);
         var loopLabel, ls' := ls.GenerateLoopLabel();
-        var b :- ResolveStmt(body, rs, ls');
+        var b :- ResolveStmt(body, prs, ls');
         r := LabeledStmt(loopLabel, Loop(invs, b));
-        assert stmt.WellFormed(rs.b3, ls.varMap.Keys, ls.LabelSet(), ls.loopLabel.Some?) by {
-          assert forall ae <- invariants :: ae.WellFormed(rs.b3, ls.varMap.Keys);
+        assert stmt.WellFormed(prs.ers.b3, ls.varMap.Keys, ls.LabelSet(), ls.loopLabel.Some?) by {
+          assert forall ae <- invariants :: ae.WellFormed(prs.ers.b3, ls.varMap.Keys);
           assert ls.varMap.Keys == ls'.varMap.Keys;
           assert ls.LabelSet() == ls'.LabelSet();
           assert ls'.loopLabel.Some?;
-          assert body.WellFormed(rs.b3, ls'.varMap.Keys, ls'.LabelSet(), ls'.loopLabel.Some?);
+          assert body.WellFormed(prs.ers.b3, ls'.varMap.Keys, ls'.LabelSet(), ls'.loopLabel.Some?);
         }
 
       case LabeledStmt(lbl, body) =>
@@ -382,7 +543,7 @@ module Resolver {
           return Failure("duplicate label name: " + lbl);
         }
         var l := new Label(lbl);
-        var b :- ResolveStmt(body, rs, ls.AddLabel(lbl, l));
+        var b :- ResolveStmt(body, prs, ls.AddLabel(lbl, l));
         r := LabeledStmt(l, b);
 
       case Exit(maybeLabel) =>
@@ -401,24 +562,24 @@ module Resolver {
         r := Exit(ls.returnLabel);
 
       case Probe(expr) =>
-        var e :- ResolveExpr(expr, rs, ls.varMap);
+        var e :- ResolveExpr(expr, prs.ers, ls.varMap);
         r := Probe(e);
     }
     return Success(r);
   }
 
-  method ResolveCallStmt(stmt: Raw.Stmt, rs: ResolverState, ls: LocalResolverState) returns (result: Result<Stmt, string>)
-    requires stmt.Call? && rs.Valid()
-    ensures result.Success? ==> stmt.WellFormed(rs.b3, ls.varMap.Keys, ls.LabelSet(), ls.loopLabel.Some?)
+  method ResolveCallStmt(stmt: Raw.Stmt, prs: ProcResolverState, ls: LocalResolverState) returns (result: Result<Stmt, string>)
+    requires stmt.Call? && prs.Valid()
+    ensures result.Success? ==> stmt.WellFormed(prs.ers.b3, ls.varMap.Keys, ls.LabelSet(), ls.loopLabel.Some?)
     ensures result.Success? ==> result.value.WellFormed()
   {
     var Call(name, args) := stmt;
 
-    if name !in rs.procMap {
+    if name !in prs.procMap {
       return Failure("call to undeclared procedure: " + name);
     }
-    var proc := rs.procMap[name];
-    var rawProc :| rawProc in rs.b3.procedures && rawProc.name == name;
+    var proc := prs.procMap[name];
+    var rawProc :| rawProc in prs.ers.b3.procedures && rawProc.name == name;
     assert |rawProc.parameters| == |proc.Parameters|;
 
     if |args| != |proc.Parameters| {
@@ -429,14 +590,14 @@ module Resolver {
     var aa: seq<CallArgument> := [];
     for n := 0 to |args|
       invariant forall i :: 0 <= i < n ==> args[i].mode == rawProc.parameters[i].mode
-      invariant forall i :: 0 <= i < n ==> args[i].arg.WellFormed(rs.b3, ls.varMap.Keys)
+      invariant forall i :: 0 <= i < n ==> args[i].arg.WellFormed(prs.ers.b3, ls.varMap.Keys)
       invariant |aa| == n
       invariant forall i :: 0 <= i < n ==> aa[i].CorrespondingMode() == proc.Parameters[i].mode && aa[i].WellFormed()
     {
       if args[n].mode != proc.Parameters[n].mode {
         return Failure("mismatched parameter mode in call to procedure " + name);
       }
-      var e :- ResolveExpr(args[n].arg, rs, ls.varMap);
+      var e :- ResolveExpr(args[n].arg, prs.ers, ls.varMap);
       var ca;
       if args[n].mode == Raw.In {
         ca := InArgument(e);
@@ -461,8 +622,8 @@ module Resolver {
       Block([Assume(expr), stmt])
   }
 
-  method ResolveExpr(expr: Raw.Expr, rs: ResolverState, varMap: map<string, Variable>) returns (result: Result<Expr, string>)
-    ensures result.Success? ==> expr.WellFormed(rs.b3, varMap.Keys)
+  method ResolveExpr(expr: Raw.Expr, ers: ExprResolverState, varMap: map<string, Variable>) returns (result: Result<Expr, string>)
+    ensures result.Success? ==> expr.WellFormed(ers.b3, varMap.Keys)
     ensures result.Success? ==> result.value.WellFormed()
   {
     var r: Expr;
@@ -472,7 +633,7 @@ module Resolver {
       case ILiteral(value) =>
         r := ILiteral(value);
       case CustomLiteral(s, typeName) =>
-        var typ :- ResolveType(typeName, rs.typeMap);
+        var typ :- ResolveType(typeName, ers.typeMap);
         if typ == BoolType || typ == IntType {
           return Failure("custom literal is not allowed for a built-in type: " + Ast.CustomLiteralToString(s, typeName));
         }
@@ -486,69 +647,69 @@ module Resolver {
         if |args| != op.ArgumentCount() {
           return Failure("operator " + op.ToString() + " expects " + Int2String(op.ArgumentCount()) + " arguments, got " + Int2String(|args|));
         }
-        var resolvedArgs :- ResolveExprList(args, rs, varMap);
+        var resolvedArgs :- ResolveExprList(args, ers, varMap);
         r := OperatorExpr(op, resolvedArgs);
       case FunctionCallExpr(name, args) =>
-        var func := new Function(name); // TODO: This is bogus. It should instead look up the already declared function
-        var resolvedArgs :- ResolveExprList(args, rs, varMap);
+        var func := new Function(name, []); // TODO: This is bogus. It should instead look up the already declared function
+        var resolvedArgs :- ResolveExprList(args, ers, varMap);
         r := FunctionCallExpr(func, resolvedArgs);
       case LabeledExpr(name, body) =>
         var lbl := new Label(name);
-        var b :- ResolveExpr(body, rs, varMap);
+        var b :- ResolveExpr(body, ers, varMap);
         r := LabeledExpr(lbl, b);
       case LetExpr(name, typeName, rhs, body) =>
         if !Raw.LegalVariableName(name) {
           return Failure("illegal variable name: " + name);
         }
-        var typ :- ResolveType(typeName, rs.typeMap);
+        var typ :- ResolveType(typeName, ers.typeMap);
         var letVariable := new LocalVariable(name, false, typ);
-        var rRhs :- ResolveExpr(rhs, rs, varMap);
+        var rRhs :- ResolveExpr(rhs, ers, varMap);
         var varMap' := varMap[name := letVariable];
         assert varMap'.Keys == varMap.Keys + {name};
-        var rBody :- ResolveExpr(body, rs, varMap');
+        var rBody :- ResolveExpr(body, ers, varMap');
         r := LetExpr(letVariable, rRhs, rBody);
       case QuantifierExpr(univ, name, typeName, patterns, body) =>
         if !Raw.LegalVariableName(name) {
           return Failure("illegal variable name: " + name);
         }
-        var typ :- ResolveType(typeName, rs.typeMap);
+        var typ :- ResolveType(typeName, ers.typeMap);
         var quantifiedVariable := new LocalVariable(name, false, typ);
         var varMap' := varMap[name := quantifiedVariable];
         assert varMap'.Keys == varMap.Keys + {name};
-        var b :- ResolveExpr(body, rs, varMap');
-        var trs :- ResolvePatterns(patterns, rs, varMap');
+        var b :- ResolveExpr(body, ers, varMap');
+        var trs :- ResolvePatterns(patterns, ers, varMap');
         r := QuantifierExpr(univ, quantifiedVariable, trs, b);
     }
     return Success(r);
   }
 
-  method ResolveExprList(exprs: seq<Raw.Expr>, rs: ResolverState, varMap: map<string, Variable>) returns (result: Result<seq<Expr>, string>)
-    ensures result.Success? ==> forall expr <- exprs :: expr.WellFormed(rs.b3, varMap.Keys)
+  method ResolveExprList(exprs: seq<Raw.Expr>, ers: ExprResolverState, varMap: map<string, Variable>) returns (result: Result<seq<Expr>, string>)
+    ensures result.Success? ==> forall expr <- exprs :: expr.WellFormed(ers.b3, varMap.Keys)
     ensures result.Success? ==> |result.value| == |exprs|
     ensures result.Success? ==> forall expr <- result.value :: expr.WellFormed()
   {
     var resolvedExprs := [];
     for n := 0 to |exprs|
-      invariant forall expr <- exprs[..n] :: expr.WellFormed(rs.b3, varMap.Keys)
+      invariant forall expr <- exprs[..n] :: expr.WellFormed(ers.b3, varMap.Keys)
       invariant |resolvedExprs| == n
       invariant forall expr: Expr <- resolvedExprs :: expr.WellFormed()
     {
-      var r :- ResolveExpr(exprs[n], rs, varMap);
+      var r :- ResolveExpr(exprs[n], ers, varMap);
       resolvedExprs := resolvedExprs + [r];
     }
     return Success(resolvedExprs);
   }
 
-  method ResolvePatterns(patterns: seq<Raw.Pattern>, rs: ResolverState, varMap: map<string, Variable>) returns (result: Result<seq<Pattern>, string>)
-    ensures result.Success? ==> forall tr <- patterns :: tr.WellFormed(rs.b3, varMap.Keys)
+  method ResolvePatterns(patterns: seq<Raw.Pattern>, ers: ExprResolverState, varMap: map<string, Variable>) returns (result: Result<seq<Pattern>, string>)
+    ensures result.Success? ==> forall tr <- patterns :: tr.WellFormed(ers.b3, varMap.Keys)
     ensures result.Success? ==> forall tr <- result.value :: tr.WellFormed()
   {
     var resolvedPatterns := [];
     for n := 0 to |patterns|
-      invariant forall tr <- patterns[..n] :: tr.WellFormed(rs.b3, varMap.Keys)
+      invariant forall tr <- patterns[..n] :: tr.WellFormed(ers.b3, varMap.Keys)
       invariant forall tr: Pattern <- resolvedPatterns :: tr.WellFormed()
     {
-      var exprs :- ResolveExprList(patterns[n].exprs, rs, varMap);
+      var exprs :- ResolveExprList(patterns[n].exprs, ers, varMap);
       resolvedPatterns := resolvedPatterns + [Pattern(exprs)];
     }
     return Success(resolvedPatterns);
